projects/MyGIT.v
@@ -1,0 +1,591 @@
+Require Import Coq.Arith.PeanoNat.
+Require Import Coq.Bool.Bool.
+Require Import Coq.micromega.Lia.
+Require Import Coq.Lists.List.
+Require Import DschingisKhan.pure.MyStructures.
+Require Import DschingisKhan.pure.MyUtilities.
+
+Module Smullyan's_Goedel's_Incompleteness_Theorems.
+
+  Import ListNotations MyUtilities MyEnsemble.
+
+  Section Chapter1.
+
+  Class GoedelianLanguage (mathcalE : Type) : Type :=
+    { enum_mathcalE : nat -> mathcalE
+    ; mathcalE_is_denumerable : forall E : mathcalE, {n : nat | enum_mathcalE n = E}
+    ; isSentence : ensemble mathcalE
+    ; isProvable : ensemble mathcalE
+    ; isRefutable : ensemble mathcalE
+    ; isPredicate : ensemble mathcalE
+    ; appnat : mathcalE -> nat -> mathcalE
+    ; isTrue : ensemble mathcalE
+    ; onlyProvableIsSentence : isSubsetOf isProvable isSentence
+    ; onlyRefutableIsSentence : isSubsetOf isRefutable isSentence
+    ; appnatForPredicate : forall h : mathcalE, isPredicate h -> forall n : nat, isSentence (appnat h n)
+    ; onlyTrueIsSentence : isSubsetOf isTrue isSentence
+    }
+  .
+
+  Context (mathcalE : Type) `{mathcalE_is_goedelian : GoedelianLanguage mathcalE}.
+
+  Definition diagonalizer : nat -> nat :=
+    fun n : nat =>
+    proj1_sig (mathcalE_is_denumerable (appnat (enum_mathcalE n) n))
+  .
+
+  Local Hint Unfold diagonalizer : my_hints.
+
+  Lemma diagonalizer_diagonalizes :
+    forall n : nat,
+    forall E : mathcalE,
+    enum_mathcalE n = E ->
+    enum_mathcalE (diagonalizer n) = appnat E n.
+  Proof with eauto with *.
+    unfold diagonalizer.
+    intros n E H'.
+    subst.
+    destruct (mathcalE_is_denumerable (appnat (enum_mathcalE n) n)) as [d_n H]...
+  Qed.
+
+  Definition expressPredicate : mathcalE -> ensemble nat -> Prop :=
+    fun H : mathcalE =>
+    fun A : ensemble nat =>
+    forall n : nat,
+    isTrue (appnat H n) <-> member n A
+  .
+
+  Local Hint Unfold expressPredicate : my_hints.
+
+  Definition is_expressible : ensemble nat -> Prop :=
+    fun A : ensemble nat =>
+    exists H : mathcalE, expressPredicate H A
+  .
+
+  Local Hint Unfold is_expressible : my_hints.
+
+  Inductive StarOf : ensemble nat -> ensemble nat :=
+  | InStarOf :
+    forall ns : ensemble nat,
+    forall n : nat,
+    member (diagonalizer n) ns ->
+    member n (StarOf ns)
+  .
+
+  Local Hint Constructors StarOf : my_hints.
+
+  Definition isCorrect : Prop :=
+    isSubsetOf isProvable isTrue /\ isSubsetOf (intersection isRefutable isTrue) \emptyset
+  .
+
+  Local Hint Unfold isCorrect : my_hints.
+
+  Inductive P : ensemble nat :=
+  | InP :
+    forall n : nat,
+    isProvable (enum_mathcalE n) ->
+    member n P
+  .
+
+  Local Hint Constructors P : my_hints.
+
+  Theorem After_Goedel_with_shades_of_Tarski :
+    isCorrect ->
+    is_expressible (StarOf (completement P)) ->
+    exists E : mathcalE, isTrue E /\ ~ isProvable E.
+  Proof with eauto with *.
+    intros mathcalE_is_correct [H H_express_StarOf_complement_P].
+    destruct (mathcalE_is_denumerable H) as [n n_is_the_goedel_number_of_H].
+    assert (diagonalization_of_n_is_true_iff_n_is_in_StarOf_complement_of_P : isTrue (enum_mathcalE (diagonalizer n)) <-> member n (StarOf (completement P))).
+    { unfold expressPredicate in H_express_StarOf_complement_P.
+      rewrite (diagonalizer_diagonalizes n H n_is_the_goedel_number_of_H)...
+    }
+    assert (n_in_StarOf_complement_of_P_iff_diagonalization_of_n_is_not_Provable : member n (StarOf (completement P)) <-> ~ isProvable (enum_mathcalE (diagonalizer n))).
+    { split.
+      - intros n_in_StarOf_complement_of_P diagonalization_of_n_is_not_Provable.
+        inversion n_in_StarOf_complement_of_P as [A n' diagonalization_of_n_is_in_A A_is_complement_of_P n_is_n']; subst n'.
+        contradiction diagonalization_of_n_is_in_A...
+      - intros diagonalization_of_n_is_not_Provable.
+        constructor.
+        intros diagonalization_of_n_is_in_P.
+        contradiction diagonalization_of_n_is_not_Provable.
+        inversion diagonalization_of_n_is_in_P as [n' diagonalization_of_n_is_Provable n_is_n']; subst n'...
+    }
+    assert (diagonalization_of_n_is_not_Provable : ~ isProvable (enum_mathcalE (diagonalizer n))).
+    { intros diagonalization_of_n_is_Provable.
+      destruct mathcalE_is_correct as [Provable_implies_true Refutable_implies_false].
+      assert (diagonalization_of_n_is_True : isTrue (enum_mathcalE (diagonalizer n))) by firstorder.
+      tauto.
+    }
+    now firstorder.
+  Qed.
+
+  Definition the_first_goal : Prop :=
+    forall A : ensemble nat,
+    is_expressible A ->
+    is_expressible (StarOf A)
+  .
+
+  Definition the_second_goal : Prop :=
+    forall A : ensemble nat,
+    is_expressible A ->
+    is_expressible (completement A)
+  .
+
+  Definition the_third_goal : Prop :=
+    is_expressible P
+  .
+
+  Definition isGoedelSentence : mathcalE -> ensemble nat -> Prop :=
+    fun E : mathcalE =>
+    fun A : ensemble nat =>
+    exists n : nat, enum_mathcalE n = E /\ (isTrue E <-> member n A)
+  .
+
+  Lemma A_Diagonal_Lemma_a :
+    forall A : ensemble nat,
+    is_expressible (StarOf A) ->
+    exists E : mathcalE, isGoedelSentence E A.
+  Proof with eauto with *.
+    intros A [H H_express_StarOf_A].
+    destruct (mathcalE_is_denumerable H) as [n g_H_is_n].
+    exists (appnat H n).
+    assert (H_n_is_true_iff_d_n_is_in_A : isTrue (appnat H n) <-> member (diagonalizer n) A).
+    { split.
+      - intros H_n_is_true.
+        assert (n_is_in_StarOfA : member n (StarOf A)) by firstorder.
+        inversion n_is_in_StarOfA as [A' n' d_n_is_in_A A_is_A' n_is_n']; subst...
+      - intros d_n_is_in_A.
+        apply H_express_StarOf_A...
+    }
+    assert (d_n_is_g_H_n : enum_mathcalE (diagonalizer n) = appnat H n).
+    { unfold diagonalizer.
+      rewrite (proj2_sig (mathcalE_is_denumerable (appnat (enum_mathcalE n) n))), g_H_is_n...
+    }
+    now firstorder.
+  Qed.
+
+  Lemma A_Diagonal_Lemma_b :
+    the_first_goal ->
+    forall A : ensemble nat,
+    is_expressible A ->
+    exists E : mathcalE, isGoedelSentence E A.
+  Proof with eauto with *.
+    intros the_first_goal_holds A A_is_expressible.
+    apply A_Diagonal_Lemma_a, the_first_goal_holds...
+  Qed.
+
+  Inductive T : ensemble nat :=
+  | InT :
+    forall n : nat,
+    isTrue (enum_mathcalE n) ->
+    member n T
+  .
+
+  Local Hint Constructors T : my_hints.
+
+  Theorem there_is_no_GoedelSentence_of_complement_of_T :
+    ~ (exists E : mathcalE, isGoedelSentence E (completement T)).
+  Proof with (tauto || eauto with *).
+    intros [E [n [n_is_g_E E_is_true_iff_n_is_in_complement_T]]].
+    assert (E_is_true_iff_n_is_not_in_T : isTrue E <-> ~ member n T) by firstorder.
+    assert (E_is_true_iff_n_is_in_T : isTrue E <-> member n T)...
+    split.
+    - intros E_is_true.
+      constructor.
+      rewrite n_is_g_E...
+    - intros n_is_inT.
+      inversion n_is_inT as [n' E_is_true n_is_n']; subst n'.
+      rewrite <- n_is_g_E...
+  Qed.
+
+  Theorem After_Tarski_1 :
+    ~ is_expressible (StarOf (completement T)).
+  Proof with eauto with *.
+    intros StarOf_T_is_expressible.
+    destruct (A_Diagonal_Lemma_a (completement T) StarOf_T_is_expressible) as [H H_is_GoedelSentence_for_complement_of_T].
+    contradiction (there_is_no_GoedelSentence_of_complement_of_T)...
+  Qed.
+
+  Theorem After_Tarski_2 :
+    the_first_goal->
+    ~ is_expressible (completement T).
+  Proof with eauto.
+    intros the_first_goal_holds completement_of_T_is_expressible.
+    apply After_Tarski_1, the_first_goal_holds...
+  Qed.
+
+  Theorem After_Tarski_3 :
+    the_first_goal ->
+    the_second_goal ->
+    ~ is_expressible T.
+  Proof with eauto.
+    intros the_first_goal_holds the_second_goal_holds T_is_expressible.
+    apply (After_Tarski_2 the_first_goal_holds), the_second_goal_holds...
+  Qed.
+
+  End Chapter1.
+
+  Section Chapter2.
+
+  Definition vr : Set :=
+    nat
+  .
+
+  Inductive tm : Set :=
+  | ivar_tm : vr -> tm
+  | zero_tm : tm
+  | succ_tm : tm -> tm
+  | plus_tm : tm -> tm -> tm
+  | mult_tm : tm -> tm -> tm
+  | expo_tm : tm -> tm -> tm
+  .
+
+  Inductive form : Set :=
+  | eqn_form : tm -> tm -> form
+  | leq_form : tm -> tm -> form
+  | neg_form : form -> form
+  | imp_form : form -> form -> form
+  | all_form : vr -> form -> form
+  .
+
+  Local Hint Resolve Nat.eqb_eq : my_hints.
+
+  Local Hint Resolve Nat.eqb_neq : my_hints.
+
+  Lemma vr_eq_dec :
+    forall x1 : vr,
+    forall x2 : vr,
+    {x1 = x2} + {x1 <> x2}.
+  Proof.
+    apply Nat.eq_dec.
+  Qed.
+
+  Ltac simpl_vr_eq_dec :=
+    simpl;
+    repeat (repeat split; intro);
+    match goal with
+    | H : (if vr_eq_dec ?x1 ?x2 then ?casel else ?caser) = ?rhs |- _ =>
+      destruct (vr_eq_dec x1 x2); try now firstorder
+    | H : ?lhs = (if vr_eq_dec ?x1 ?x2 then ?casel else ?caser) |- _ =>
+      destruct (vr_eq_dec x1 x2); try now firstorder
+    | |- (if vr_eq_dec ?x1 ?x2 then ?casel else ?caser) = ?rhs =>
+      destruct (vr_eq_dec x1 x2); try now firstorder
+    | |- ?lhs = (if vr_eq_dec ?x1 ?x2 then ?casel else ?caser) =>
+      destruct (vr_eq_dec x1 x2); try now firstorder
+    end
+  .
+
+  Ltac auto_rewrite :=
+    repeat intro;
+    repeat (
+      rewrite in_app_iff ||
+      rewrite orb_true_iff ||
+      rewrite orb_false_iff ||
+      rewrite andb_true_iff ||
+      rewrite negb_true_iff ||
+      rewrite andb_false_iff ||
+      rewrite negb_false_iff ||
+      rewrite forallb_true_iff
+    );
+    try now firstorder
+  .
+
+  Fixpoint occursFreeIn_tm (z : vr) (t : tm) : bool :=
+    match t with
+    | ivar_tm x => if vr_eq_dec z x then true else false
+    | zero_tm => false
+    | succ_tm t1 => occursFreeIn_tm z t1
+    | plus_tm t1 t2 => occursFreeIn_tm z t1 || occursFreeIn_tm z t2
+    | mult_tm t1 t2 => occursFreeIn_tm z t1 || occursFreeIn_tm z t2
+    | expo_tm t1 t2 => occursFreeIn_tm z t1 || occursFreeIn_tm z t2
+    end
+  .
+
+  Fixpoint occursFreeIn_form (z : vr) (f : form) : bool :=
+    match f with
+    | eqn_form t1 t2 => occursFreeIn_tm z t1 || occursFreeIn_tm z t2
+    | leq_form t1 t2 => occursFreeIn_tm z t1 || occursFreeIn_tm z t2
+    | neg_form f1 => occursFreeIn_form z f1
+    | imp_form f1 f2 => occursFreeIn_form z f1 || occursFreeIn_form z f2
+    | all_form x f1 => if vr_eq_dec z x then false else occursFreeIn_form z f1
+    end
+  .
+
+  Fixpoint getFreeVars_tm (t : tm) : list vr :=
+    match t with
+    | ivar_tm x => [x]
+    | zero_tm => []
+    | succ_tm t1 => getFreeVars_tm t1
+    | plus_tm t1 t2 => getFreeVars_tm t1 ++ getFreeVars_tm t2
+    | mult_tm t1 t2 => getFreeVars_tm t1 ++ getFreeVars_tm t2
+    | expo_tm t1 t2 => getFreeVars_tm t1 ++ getFreeVars_tm t2
+    end
+  .
+
+  Theorem the_rule_of_getFreeVars_tm :
+    forall t : tm,
+    forall x : vr,
+    In x (getFreeVars_tm t) <-> occursFreeIn_tm x t = true.
+  Proof with try now eauto.
+    induction t; simpl.
+    - simpl_vr_eq_dec.
+    - split...
+    - intros x...
+    - auto_rewrite.
+    - auto_rewrite.
+    - auto_rewrite.
+  Qed.
+
+  Fixpoint getFreeVars_form (f : form) : list vr :=
+    match f with
+    | eqn_form t1 t2 => getFreeVars_tm t1 ++ getFreeVars_tm t2
+    | leq_form t1 t2 => getFreeVars_tm t1 ++ getFreeVars_tm t2
+    | neg_form f1 => getFreeVars_form f1
+    | imp_form f1 f2 => getFreeVars_form f1 ++ getFreeVars_form f2
+    | all_form x f1 => remove vr_eq_dec x (getFreeVars_form f1)
+    end
+  .
+
+  Theorem the_rule_of_getFreeVars_form :
+    forall f : form,
+    forall x : vr,
+    In x (getFreeVars_form f) <-> occursFreeIn_form x f = true.
+  Proof with try now firstorder.
+    induction f; simpl...
+    - auto_rewrite.
+      repeat (rewrite the_rule_of_getFreeVars_tm)...
+    - auto_rewrite.
+      repeat (rewrite the_rule_of_getFreeVars_tm)...
+    - auto_rewrite.
+    - intros x.
+      split.
+      + intros H.
+        assert (H0 : In x (getFreeVars_form f) /\ x <> v) by now apply (in_remove vr_eq_dec (getFreeVars_form f) x v).
+        simpl_vr_eq_dec.
+      + intros H.
+        simpl_vr_eq_dec.
+        apply in_in_remove...
+  Qed.
+
+  Definition value_assignment : Set :=
+    vr -> nat
+  .
+
+  Fixpoint eval_tm (va : value_assignment) (t : tm) : nat :=
+    match t with
+    | ivar_tm x => va x
+    | zero_tm => 0
+    | succ_tm t1 => S (eval_tm va t1)
+    | plus_tm t1 t2 => eval_tm va t1 + eval_tm va t2
+    | mult_tm t1 t2 => eval_tm va t1 * eval_tm va t2
+    | expo_tm t1 t2 => (eval_tm va t1)^(eval_tm va t2)
+    end
+  .
+
+  Lemma eval_tm_extensionality :
+    forall t : tm,
+    forall va1 : value_assignment,
+    forall va2 : value_assignment,
+    (forall x : vr, occursFreeIn_tm x t = true -> va1 x = va2 x) ->
+    eval_tm va1 t = eval_tm va2 t.
+  Proof with eauto.
+    induction t; simpl...
+    { intros va1 va2 H.
+      apply H.
+      simpl_vr_eq_dec.
+    }
+    all: intros va1 va2 H; rewrite (IHt1 va1 va2), (IHt2 va1 va2)...
+    all: intros x H0; apply H, orb_true_iff; tauto.
+  Qed.
+
+  Fixpoint eval_form (va : value_assignment) (f : form) : Prop :=
+    match f with
+    | eqn_form t1 t2 => eval_tm va t1 = eval_tm va t2
+    | leq_form t1 t2 => eval_tm va t1 <= eval_tm va t2
+    | neg_form f1 => ~ eval_form va f1
+    | imp_form f1 f2 => eval_form va f1 -> eval_form va f2
+    | all_form x f1 => forall val : nat, eval_form (fun z : vr => if vr_eq_dec x z then val else va z) f1
+    end
+  .
+
+  Lemma eval_form_extensionality :
+    forall f : form,
+    forall va1 : value_assignment,
+    forall va2 : value_assignment,
+    (forall x : vr, occursFreeIn_form x f = true -> va1 x = va2 x) ->
+    eval_form va1 f <-> eval_form va2 f.
+  Proof with (reflexivity || eauto).
+    induction f; simpl...
+    1, 2: intros va1 va2 H; rewrite (eval_tm_extensionality t va1 va2), (eval_tm_extensionality t0 va1 va2)...
+    1, 2, 3, 4: intros x H0; apply H, orb_true_iff...
+    1: intros va1 va2 H; rewrite (IHf va1 va2)...
+    1: intros va1 va2 H; rewrite (IHf1 va1 va2), (IHf2 va1 va2)...
+    1, 2: intros x H0; apply H, orb_true_iff...
+    { intros va1 va2 H.
+      enough (claim1 : forall n : nat, eval_form (fun z : vr => if vr_eq_dec v z then n else va1 z) f <->  eval_form (fun z : vr => if vr_eq_dec v z then n else va2 z) f) by firstorder.
+      intros n.
+      rewrite (IHf (fun z : vr => if vr_eq_dec v z then n else va1 z) (fun z : vr => if vr_eq_dec v z then n else va2 z))...
+      simpl_vr_eq_dec.
+      apply H.
+      simpl_vr_eq_dec.
+    }
+  Qed.
+
+  Fixpoint make_numeral (n : nat) : tm :=
+    match n with
+    | 0 => zero_tm
+    | S n => succ_tm (make_numeral n)
+    end
+  .
+
+  Lemma eval_tm_make_numeral :
+    forall n : nat,
+    forall va : value_assignment,
+    eval_tm va (make_numeral n) = n.
+  Proof with eauto.
+    induction n; simpl...
+  Qed.
+
+  Definition substitution : Set :=
+    list (vr * tm)
+  .
+
+  Fixpoint substitute_vr (sigma : substitution) (x : vr) : tm :=
+    match sigma with
+    | [] => ivar_tm x
+    | (x1, tm1) :: sigma' => if vr_eq_dec x x1 then tm1 else substitute_vr sigma' x
+    end
+  .
+
+  Fixpoint substitute_tm (sigma : substitution) (t : tm) : tm :=
+    match t with
+    | ivar_tm x => substitute_vr sigma x
+    | zero_tm => zero_tm
+    | succ_tm t1 => succ_tm (substitute_tm sigma t1)
+    | plus_tm t1 t2 => plus_tm (substitute_tm sigma t1) (substitute_tm sigma t2)
+    | mult_tm t1 t2 => mult_tm (substitute_tm sigma t1) (substitute_tm sigma t2)
+    | expo_tm t1 t2 => expo_tm (substitute_tm sigma t1) (substitute_tm sigma t2)
+    end
+  .
+
+  Theorem substitute_tm_preserves_eval_tm :
+    forall t : tm,
+    forall sigma : substitution,
+    forall va : value_assignment,
+    eval_tm (fun z : vr => eval_tm va (substitute_vr sigma z)) t = eval_tm va (substitute_tm sigma t).
+  Proof with eauto.
+    induction t; simpl...
+  Qed.
+
+  Definition getMaxNumOfFreeVars_tm (t : tm) : vr :=
+    fold_right_max_0 (getFreeVars_tm t)
+  .
+
+  Lemma getMaxNumOfFreeVars_tm_lt :
+    forall t : tm,
+    forall x : vr,
+    getMaxNumOfFreeVars_tm t < x ->
+    occursFreeIn_tm x t = false.
+  Proof with (lia || eauto).
+    unfold getMaxNumOfFreeVars_tm.
+    induction t; simpl...
+    1: simpl_vr_eq_dec...
+    all: auto_rewrite; rewrite fold_right_max_0_app in H; (split; [apply IHt1 | apply IHt2])...
+  Qed.
+
+  Definition isFreshVarIn_substitute_tm (sigma : substitution) (z : vr) (t : tm) : Prop :=
+    forallb (fun x : vr => negb (occursFreeIn_tm z (substitute_vr sigma x))) (getFreeVars_tm t) = true
+  .
+
+  Definition isFreshVarIn_substitute_form (sigma : substitution) (z : vr) (f : form) : Prop :=
+    forallb (fun x : vr => negb (occursFreeIn_tm z (substitute_vr sigma x))) (getFreeVars_form f) = true
+  .
+
+  Definition chi (sigma : substitution) (f : form) : vr :=
+    S (fold_right_max_0 (map (fun x : vr => getMaxNumOfFreeVars_tm (substitute_vr sigma x)) (getFreeVars_form f)))
+  .
+
+  Theorem the_rule_of_chi :
+    forall f : form,
+    forall sigma : substitution,
+    isFreshVarIn_substitute_form sigma (chi sigma f) f.
+  Proof with eauto.
+    assert ( claim1 :
+      forall sigma : substitution,
+      forall f : form,
+      forall x : vr,
+      occursFreeIn_form x f = true ->
+      occursFreeIn_tm (chi sigma f) (substitute_vr sigma x) = false
+    ).
+    { intros sigma f x H.
+      enough (claim1_aux1 : getMaxNumOfFreeVars_tm (substitute_vr sigma x) < chi sigma f) by now apply getMaxNumOfFreeVars_tm_lt.
+      unfold chi, fold_right_max_0.
+      enough (claim1_aux2 : fold_right max 0 (map (fun z : vr => getMaxNumOfFreeVars_tm (substitute_vr sigma z)) (getFreeVars_form f)) >= getMaxNumOfFreeVars_tm (substitute_vr sigma x)) by lia.
+      rewrite <- the_rule_of_getFreeVars_form in H.
+      apply fold_right_max_0_in, in_map_iff...
+    }
+    unfold isFreshVarIn_substitute_form.
+    repeat auto_rewrite.
+    apply claim1, the_rule_of_getFreeVars_form...
+  Qed.
+
+  Fixpoint substitute_form (sigma : substitution) (f : form) : form :=
+    match f with
+    | eqn_form t1 t2 => eqn_form (substitute_tm sigma t1) (substitute_tm sigma t2)
+    | leq_form t1 t2 => leq_form (substitute_tm sigma t1) (substitute_tm sigma t2)
+    | neg_form f1 => neg_form (substitute_form sigma f1)
+    | imp_form f1 f2 => imp_form (substitute_form sigma f1) (substitute_form sigma f2)
+    | all_form x f1 =>
+      let z : vr := chi sigma f in
+      all_form z (substitute_form ((x, ivar_tm z) :: sigma) f1)
+    end
+  .
+
+  Theorem substitute_form_preserves_eval_form :
+    forall f : form,
+    forall sigma : substitution,
+    forall va : value_assignment,
+    eval_form (fun z : vr => eval_tm va (substitute_vr sigma z)) f <-> eval_form va (substitute_form sigma f).
+  Proof with (reflexivity || eauto).
+    induction f; simpl; intros sigma va...
+    1, 2: repeat (rewrite substitute_tm_preserves_eval_tm)...
+    1: rewrite IHf...
+    1: rewrite IHf1, IHf2...
+    1: enough (claim1 : forall n : nat, eval_form (fun z : vr => if vr_eq_dec v z then n else eval_tm va (substitute_vr sigma z)) f <-> eval_form (fun z : vr => if vr_eq_dec (chi sigma (all_form v f)) z then n else va z) (substitute_form ((v, ivar_tm (chi sigma (all_form v f))) :: sigma) f)) by firstorder.
+    intros n.
+    rewrite <- (IHf ((v, ivar_tm (chi sigma (all_form v f))) :: sigma) (fun z : vr => if vr_eq_dec (chi sigma (all_form v f)) z then n else va z)).
+    apply eval_form_extensionality.
+    intros x H.
+    simpl.
+    destruct (vr_eq_dec v x).
+    - destruct (vr_eq_dec x v).
+      + simpl.
+        now destruct (vr_eq_dec (chi sigma (all_form v f)) (chi sigma (all_form v f))).
+      + contradiction n0...
+    - destruct (vr_eq_dec x v).
+      + contradiction n0...
+      + apply eval_tm_extensionality.
+        intros x' H0.
+        simpl_vr_eq_dec.
+        subst.
+        assert (claim1_aux1 : isFreshVarIn_substitute_form sigma (chi sigma (all_form v f)) (all_form v f)) by apply the_rule_of_chi.
+        unfold isFreshVarIn_substitute_form in claim1_aux1.
+        rewrite forallb_true_iff in claim1_aux1.
+        enough (claim1_aux2 : negb (occursFreeIn_tm (chi sigma (all_form v f)) (substitute_vr sigma x)) = true) by now rewrite H0 in claim1_aux2.
+        apply claim1_aux1, the_rule_of_getFreeVars_form.
+        simpl_vr_eq_dec.
+  Qed.
+
+  Lemma substitute_tm_make_numeral :
+    forall n : nat,
+    forall sigma : substitution,
+    substitute_tm sigma (make_numeral n) = make_numeral n.
+  Proof with eauto.
+    induction n; simpl; intros sigma...
+    rewrite (IHn sigma)...
+  Qed.
+
+  End Chapter2.
+
+End Smullyan's_Goedel's_Incompleteness_Theorems.
